DeanLean/Cpp/Tests/Numeric.lean
@@ -1,3 +1,4 @@
+import DeanLean.Basic
 import DeanLean.Cpp.Code.Numeric
 
 namespace Cpp.Numeric.Tests
@@ -128,31 +129,31 @@ end Cpp.Numeric.Tests
 
 namespace Cpp
 
-def negative_never_equals_unsigned_test :=
+Test negative_never_equals_unsigned :=
   show cmp_equal (Int8.mk' (-1)) (0 : UInt8) = false from rfl
 
-def negative_less_than_unsigned_test :=
+Test negative_less_than_unsigned :=
   show cmp_less (Int8.mk' (-1)) (0 : UInt8) = true from rfl
 
-def cmp_equal_symmetric_test :=
+Test cmp_equal_symmetric :=
   show cmp_equal (42 : UInt32) (42 : UInt32) = cmp_equal (42 : UInt32) (42 : UInt32) from rfl
 
-def cmp_less_irreflexive_test :=
+Test cmp_less_irreflexive :=
   show cmp_less (42 : UInt32) (42 : UInt32) = false from rfl
 
-def cmp_less_asymmetric_test :=
+Test cmp_less_asymmetric :=
   show cmp_less (10 : UInt32) (20 : UInt32) = true from rfl
 
-def in_range_min_test :=
+Test in_range_min :=
   show in_range UInt8 (NumericLimits.min : UInt8) = true from rfl
 
-def in_range_max_test :=
+Test in_range_max :=
   show in_range UInt8 (NumericLimits.max : UInt8) = true from rfl
 
-def negative_not_in_unsigned_range_test :=
+Test negative_not_in_unsigned_range :=
   show in_range UInt8 (Int8.mk' (-1)) = false from rfl
 
-def lowest_eq_min_for_integers_test :=
+Test lowest_eq_min_for_integers :=
   show IntPromotable.toInt (NumericLimits.lowest : UInt8) = IntPromotable.toInt (NumericLimits.min : UInt8) from rfl
 
 end Cpp
