DeanLean/Cpp/Tests/Optional.lean
@@ -1,3 +1,4 @@
+import DeanLean.Basic
 import DeanLean.Cpp.Code.Optional
 
 namespace Cpp.Optional.Tests
@@ -63,24 +64,24 @@ end Cpp.Optional.Tests
 
 namespace Cpp.Optional
 
-def monad_left_identity_test :=
+Test monad_left_identity :=
   show (pure 5 : Optional Nat) >>= Optional.some = Optional.some 5 from rfl
 
-def monad_right_identity_test :=
+Test monad_right_identity :=
   show (Optional.some 5) >>= (pure · : Nat → Optional Nat) = Optional.some 5 from rfl
 
-def monad_associativity_test :=
+Test monad_associativity :=
   show ((Optional.some 3) >>= (fun n => Optional.some (n + 1))) >>= (fun n => Optional.some (n * 2))
     = (Optional.some 3) >>= (fun n => (fun n => Optional.some (n + 1)) n >>= (fun n => Optional.some (n * 2))) from rfl
 
-def transform_compose_test :=
+Test transform_compose :=
   show ((Optional.some 3).transform (· + 1)).transform (· * 2)
     = (Optional.some 3).transform ((· * 2) ∘ (· + 1)) from rfl
 
-def transform_id_test :=
+Test transform_id :=
   show (Optional.some 5).transform id = Optional.some 5 from rfl
 
-def or_else_and_then_nullopt_test :=
+Test or_else_and_then_nullopt :=
   show ((Optional.nullopt : Optional Nat).or_else (fun () => Optional.some 5)).and_then (fun n => Optional.some (n + 1))
     = ((fun () => Optional.some 5) ()).and_then (fun n => Optional.some (n + 1)) from rfl
 
